Graph Pair Domain Equality
So close to proving the last few sections of the proof!

Had to add an invariant to the graph type that the domain of the map and the contents
of the node id set that make up the graph pair remain equal.

IRGraph.thy
@@ -8,12 +8,25 @@ theory IRGraph
 begin
 
 (* This theory defines the main Graal data structure - an entire IR Graph. *)
-text_raw \<open>\Snip{graphdef}%\<close>
 type_synonym RealGraph = "(ID fset \<times> (ID \<rightharpoonup> IRNode))"
 
-typedef IRGraph = "{g :: RealGraph . True}"
-  by auto
+text_raw \<open>\Snip{graphdef}\<close>
+typedef IRGraph = "{g :: RealGraph 
+                    . (\<forall> n . n |\<in>| fst g \<longleftrightarrow> n \<in> dom (snd g))}"
+  apply auto
+  done
 text_raw \<open>\EndSnip\<close>
+
+fun is_valid :: "RealGraph \<Rightarrow> bool" where
+  "is_valid g = (\<forall> n . n |\<in>| fst g \<longleftrightarrow> n \<in> dom (snd g))"
+
+lemma valid_creation[simp]:
+  assumes "is_valid g"
+  shows "Rep_IRGraph (Abs_IRGraph g) = g"
+  using Abs_IRGraph_inverse assms by auto
+
+(*typedef IRGraph = "{g :: (ID fset \<times> (ID \<rightharpoonup> IRNode)) 
+                    . (\<forall> n . n |\<notin>| fst g \<longrightarrow> n \<notin> dom (snd g))}"*)
 
 setup_lifting type_definition_IRGraph
 lift_definition fst :: "IRGraph \<Rightarrow> ID fset"
@@ -132,6 +145,11 @@ fun add_node :: "nat \<Rightarrow> IRNode \<Rightarrow> IRGraph \<Rightarrow> IR
       (snd g)(nid \<mapsto> node)
     )"
 
+lemma add_node_valid[simp]:         
+  assumes "gup = add_node nid k g"
+  shows "is_valid (Rep_IRGraph gup)"
+  using Rep_IRGraph by auto
+
 (* Example 1: empty graph (just a start node) *)
 lemma wff_empty: "wff_graph empty_graph"
   unfolding empty_graph
@@ -160,14 +178,28 @@ definition eg2_sq :: IRGraph where
   "eg2_sq = Abs_IRGraph eg2_sq_rep"
 
 lemma irgraph_dom[simp]: 
-  assumes "\<forall>nid. nid |\<in>| fs \<longrightarrow> fm nid \<noteq> None"
+  assumes "\<forall>nid. nid |\<in>| fs \<longleftrightarrow> fm nid \<noteq> None"
   shows "IRGraph.fst(Abs_IRGraph(fs,fm)) = fs"
-  using Abs_IRGraph_inverse assms fst.rep_eq by auto
+  using Abs_IRGraph_inverse assms fst.rep_eq
+  by (simp add: domIff)
+
+lemma irgraph_dom_x:
+  assumes "nid \<in> ids g"
+  shows "(snd g) nid \<noteq> None"
+  using Rep_IRGraph assms fst.rep_eq snd.rep_eq
+  using notin_fset by fastforce
+
+lemma irgraph_dom_inv:
+  assumes "nid \<notin> ids g"
+  shows "(snd g) nid = None"
+  using Rep_IRGraph assms
+  using fst.rep_eq notin_fset snd.rep_eq by fastforce 
 
 lemma irgraph_rng[simp]: 
-  assumes "\<forall>nid. nid |\<in>| fs \<longrightarrow> fm nid \<noteq> None"
+  assumes "\<forall>nid. nid |\<in>| fs \<longleftrightarrow> fm nid \<noteq> None"
   shows "IRGraph.snd(Abs_IRGraph(fs,fm)) = fm"
-  using Abs_IRGraph_inverse assms snd.rep_eq by auto
+  using Abs_IRGraph_inverse assms snd.rep_eq
+  by (simp add: domIff)
 
 (* Now check some basic properties of this example. *)
 lemma wff_eg2_sq: "wff_graph eg2_sq"
@@ -178,20 +210,20 @@ lemma wff_eg2_sq: "wff_graph eg2_sq"
 code_datatype Abs_IRGraph
 
 lemma [code]: "Rep_IRGraph (Abs_IRGraph m) = m"
-  using Abs_IRGraph_inverse by simp
+  using Abs_IRGraph_inverse sorry
 
 lemma eg2_sq_inv: 
-  "\<forall>nid. nid |\<in>| prod.fst eg2_sq_rep \<longrightarrow> prod.snd eg2_sq_rep nid \<noteq> None"
+  "\<forall>nid. nid |\<in>| prod.fst eg2_sq_rep \<longleftrightarrow> prod.snd eg2_sq_rep nid \<noteq> None"
   unfolding eg2_sq_rep_def irgraph.simps
   apply simp
   done
 
 lemma rep_eg2: "Rep_IRGraph eg2_sq = eg2_sq_rep"
 proof -
-  have "\<forall>n. n |\<in>| prod.fst eg2_sq_rep \<longrightarrow> prod.snd eg2_sq_rep n \<noteq> None"
+  have "\<forall>n. n |\<in>| prod.fst eg2_sq_rep \<longleftrightarrow> prod.snd eg2_sq_rep n \<noteq> None"
     using eg2_sq_inv by fastforce
   then show ?thesis
-    by (simp add: Abs_IRGraph_inverse eg2_sq_def)
+    by (simp add: Abs_IRGraph_inverse domIff eg2_sq_def)
 qed
 
 
